theories/itree.v
@@ -11,6 +11,8 @@ Notation "x ← y ;;; z" := (ITree.bind y (λ x : _, z))
   (at level 20, y at level 100, z at level 200) : stdpp_scope.
 Notation "y ;;;; z" := (ITree.bind y (λ _, z))
   (at level 100, z at level 200, right associativity) : stdpp_scope.
+Global Instance eqit_false_true_rewrite {R E} r : RewriteRelation (@eqit E R R r false true) := { }.
+Global Instance eqit_true_false_rewrite {R E} r : RewriteRelation (@eqit E R R r true false) := { }.
 
 
 Inductive moduleE (EV S : Type) : Type → Type :=
@@ -48,6 +50,7 @@ Inductive mod_itree_step EV S : (itree (moduleE EV S) unit * S) → option EV �
 .
 
 Definition mod_itree EV S := Mod (mod_itree_step EV S).
+Global Hint Transparent mod_itree : tstep.
 
 Global Instance itree_vis_no_all EV S: VisNoAll (mod_itree EV S).
 Proof. move => *. invert_all @m_step; naive_solver. Qed.
@@ -321,8 +324,15 @@ Global Instance steps_impl_itree_proper EV S b1 b2:
   Proper ((prod_relation (eqit eq b1 b2) (=)) ==> steps_impl_eutt_rel b1 b2 ==> impl) (steps_impl (mod_itree EV S)).
 Proof. move => [??] [??] [/= Heq ->] ?? Hf ?. by apply: (steps_impl_eutt_mono _ (_, _)). Qed.
 
+Global Instance steps_impl_itree_proper_flip EV S b1 b2:
+  Proper ((prod_relation (eqit eq b1 b2) (=)) ==> flip (steps_impl_eutt_rel b2 b1) ==> flip impl) (steps_impl (mod_itree EV S)).
+Proof.
+  move => [??] [??] [/= Heq ->] ?? Hf ?. apply: (steps_impl_eutt_mono _ (_, _)); [done..|].
+  apply eqit_flip. by apply: eqit_mon; [..|done].
+Qed.
+
 Lemma steps_spec_eutt_mono {EV S} t' σ κ Pσ Pσ' b1 b2:
-  (prod_relation (eqit eq b1 b2) (=) ==> iff)%signature Pσ Pσ' →
+  (prod_relation (eqit eq b1 b2) (=) ==> impl)%signature Pσ Pσ' →
   σ -{ mod_itree EV S, κ }->ₛ Pσ →
   eqit eq b1 b2 σ.1 t' →
   (t', σ.2) -{ mod_itree EV S, κ }->ₛ Pσ'.
@@ -408,13 +418,14 @@ Proof.
   move => [??] [??] [/= Heq ->] ?? -> ?? Hf.
   split => ?.
   all: apply: (steps_spec_eutt_mono _ (_, _)); [try done| done |].
+  - move => ????. eapply Hf; [|done]. done.
   - done.
-  - move => ?? [??]. symmetry. apply Hf. split; [|done]. apply eqit_flip. by apply: eqit_mon; [..|done].
+  - move => ?? [??] ?. eapply Hf; [|done]. split; [|done]. apply eqit_flip. by apply: eqit_mon; [..|done].
   - apply eqit_flip. by apply: eqit_mon; [..|done].
 Qed.
 
 Lemma tnhas_trace_eutt_mono {EV S} t t' s κs Pσ Pσ' b1 n:
-  (prod_relation (eqit eq b1 false) (=) ==> iff)%signature Pσ Pσ' →
+  (prod_relation (eqit eq b1 false) (=) ==> impl)%signature Pσ Pσ' →
   (t, s) ~{ mod_itree EV S, κs, n }~>ₜ Pσ →
   eqit eq b1 false t t' →
   (t', s) ~{ mod_itree EV S, κs, n }~>ₜ Pσ'.
@@ -479,10 +490,17 @@ Proof.
   - move => *. subst. done.
 Qed.
 
-Lemma thas_trace_eutt_mono {EV S} t t' s κs Pσ Pσ':
-  (prod_relation (eutt eq) (=) ==> iff)%signature Pσ Pσ' →
+Global Instance tnhas_trace_itree_proper EV S b1:
+  Proper ((prod_relation (eqit eq b1 false) (=)) ==> (=) ==> (=) ==> (prod_relation (eqit eq b1 false) (=) ==> impl) ==> impl) (tnhas_trace (mod_itree EV S)).
+Proof.
+  move => [??] [??] [/= Heq ->] ?? -> ?? -> ?? Hf ?.
+  apply: tnhas_trace_eutt_mono; [try done| done |done].
+Qed.
+
+Lemma thas_trace_eutt_mono {EV S} t t' s κs Pσ Pσ' b1 b2:
+  (prod_relation (eqit eq b1 b2) (=) ==> impl)%signature Pσ Pσ' →
   (t, s) ~{ mod_itree EV S, κs }~>ₜ Pσ →
-  t ≈ t' →
+  eqit eq b1 b2 t t' →
   (t', s) ~{ mod_itree EV S, κs }~>ₜ Pσ'.
 Proof.
   move => HP /thas_trace_n[n Ht] Heq.
@@ -496,11 +514,10 @@ Proof.
     apply: thas_trace_under_tall; [done..|] => ? [??]. tend.
     eapply HP; [|done]. split; [|done] => /=. rewrite (itree_eta t) Hot (itree_eta t') Hot'. done.
   - move => m1 m2 [REL|//] t t' n κs s IHn Ht Hot Hot'. rewrite -/(eqit _ _ _) in REL.
-    apply: thas_trace_Tau'; [done|].
     move: Ht => /(tnhas_trace_Tau_inv' _ _ _ _ _)Ht. specialize (Ht _ ltac:(done)).
     apply: thas_trace_under_tall; [done..|] => ? /= [[??]|[?[??]]].
-    + tend. eapply HP; [|done]. split => //=. by rewrite (itree_eta t) Hot tau_eutt REL.
-    + apply: IHn; [done|done| |done]. by rewrite REL.
+    + tend. eapply HP; [|done]. split => //=. rewrite (itree_eta t) Hot (itree_eta t') Hot'. by apply eqit_Tau.
+    + apply: thas_trace_Tau'; [done|]. apply: IHn; [done|done| |done]. done.
   - move => u e k1 k2 Hu t t' n κs s IHn Ht Hot Hot'.
     thas_trace_inv Ht. {
       tend. eapply HP; [|done]. split; [|done] => /=. rewrite (itree_eta t) Hot (itree_eta t') Hot'.
@@ -533,52 +550,63 @@ Proof.
     move: Ht => /(tnhas_trace_Tau_inv' _ _ _ _ _ _)Ht. specialize (Ht _ ltac:(done)).
     apply: thas_trace_under_tall; [done..|] => ? /= [[??]|[?[??]]].
     + tend. eapply HP; [|done]. split; [|done] => /=. subst.
-      move: REL => /fold_eqitF REL. specialize (REL _ _ ltac:(done) ltac:(done)). rewrite -REL.
-      by rewrite (itree_eta t) Hot tau_eutt.
+      move: REL => /fold_eqitF REL. specialize (REL _ _ ltac:(done) ltac:(done)).
+      destruct b1 => //. rewrite (itree_eta t) Hot. by apply eqit_Tau_l.
     + apply: IH => //. apply: tnhas_trace_mono; [done..| by apply: ti_lt_impl_le |done].
   - move => ot1 t2 ? REL IH t t' n κs s IHn Ht Hot Hot'.
     tstep_None; [by econs|] => ? ->. by apply: IH.
 Qed.
 
 Global Instance mod_itree_proper EV S b1 b2:
-  Proper ((prod_relation (eqit eq b1 b2) (=)) ==> (=) ==> (prod_relation (eutt eq) (=) ==> iff) ==> iff) (thas_trace (mod_itree EV S)).
+  Proper ((prod_relation (eqit eq b1 b2) (=)) ==> (=) ==> (prod_relation (eqit eq b1 b2) (=) ==> iff) ==> iff) (thas_trace (mod_itree EV S)).
 Proof.
   move => [??] [??] [/= Heq ->] ?? -> ?? Hf.
   split => ?.
   all: apply: thas_trace_eutt_mono; [try done| done |].
-  - by apply: eqit_mon; [| | |done].
-  - move => ?? [??]. symmetry. by apply Hf.
-  - symmetry. by apply: eqit_mon; [| | |done].
+  - move => ????. by eapply Hf.
+  - done.
+  - move => [??] [??] [/=? ->] ?. eapply Hf; [|done]. split; [|done] => /=.
+    apply eqit_flip. by apply: eqit_mon; [..|done].
+  - apply eqit_flip. by apply: eqit_mon; [..|done].
 Qed.
 
-Definition itree_rel {E R S} (P : itree E R * S → Prop) (t : itree E R * S) : Prop :=
-  ∀ t', t.1 ≈ t' → P (t', t.2).
-Global Instance itree_rel_proper E R S P b1 b2:
-  Proper ((prod_relation (eqit eq b1 b2) (=) ==> iff)) (@itree_rel E R S P).
+Definition itree_rel {E R S} (b : bool) (P : itree E R * S → Prop) (t : itree E R * S) : Prop :=
+  ∀ t', eqit eq true b t' t.1 → P (t', t.2).
+(* Global Instance itree_rel_proper E R S P b: *)
+(*   Proper ((prod_relation (eqit eq b b) (=) ==> iff)) (@itree_rel E R S b P). *)
+(* Proof. *)
+(*   move => [x ?] [y ?] [Heq ?]. simplify_eq/=. rewrite /itree_rel /=. *)
+(*   split => ??; [rewrite -Heq | rewrite Heq]; naive_solver. *)
+(* Qed. *)
+Global Instance itree_rel_proper' E R S P b1 b2:
+  Proper ((prod_relation (eqit eq b1 b2) (=) ==> iff)) (@itree_rel E R S true P).
 Proof.
-  move => [x a] [y b] [Heq ?]. simplify_eq/=. rewrite /itree_rel /=.
-  have {}Heq : eutt eq x y. { by apply: eqit_mon; [..|done]. }
-  split => ??; [rewrite -Heq|rewrite Heq]; naive_solver.
+  move => [x ?] [y ?] [Heq ?]. simplify_eq/=. rewrite /itree_rel /=.
+  have {}Heq : x ≈ y. { by apply: eqit_mon; [..|done]. }
+  split => ??; [rewrite -Heq | rewrite Heq]; naive_solver.
 Qed.
 Typeclasses Opaque itree_rel.
 
 Lemma itree_rel_intro EV S σ κs P:
-  σ ~{mod_itree EV S, κs }~>ₜ itree_rel P →
+  σ ~{mod_itree EV S, κs }~>ₜ itree_rel true P →
   σ ~{mod_itree EV S, κs }~>ₜ P.
 Proof. move => Ht. apply: thas_trace_mono; [done|done|] => -[??] Hp. by apply: Hp. Qed.
 
 Lemma itree_rel_spec_intro EV S σ κ P:
-  σ -{mod_itree EV S, κ }->ₛ itree_rel P →
+  σ -{mod_itree EV S, κ }->ₛ itree_rel true P →
   σ -{mod_itree EV S, κ }->ₛ P.
 Proof. move => ?. apply: steps_spec_mono; [done|]. move => -[??] Hp. by apply Hp. Qed.
 
 Definition itree_impl_rel {EV S} (P : bool → option EV → (itree (moduleE EV S) () * S → Prop) → Prop) :
   bool → option EV → (itree (moduleE EV S) () * S → Prop) → Prop :=
-  λ b κ Pσ, ∀ b' (Pσ' : _ → Prop), (∀ t s, Pσ (t, s) → ∃ t', t ≈ t' ∧ Pσ' (t', s)) → P b' κ Pσ'.
-Global Instance itree_impl_rel_proper EV S b1 b2 P:
-  Proper (steps_impl_eutt_rel b1 b2) (@itree_impl_rel EV S P).
+  λ b κ Pσ, ∀ (b' : bool) (Pσ' : _ → Prop),
+      (∀ t s, Pσ (t, s) → ∃ t', eqit eq false true t t' ∧ Pσ' (t', s)) →
+      (b → b') →
+      P b' κ Pσ'.
+Global Instance itree_impl_rel_proper EV S P b:
+  Proper (steps_impl_eutt_rel false b) (@itree_impl_rel EV S P).
 Proof.
-  move => b b' κ P1 P2 HP1 Hb REL ? Pσ' HPσ'. apply: REL.
+  move => ????? HP1 ? REL ?? HPσ' ?. apply: REL. 2: naive_solver.
   move => ?? /HP1 [? [Ht /HPσ'[?[??]]]]. eexists _. split; [|done]. etrans; [|done].
   by apply: eqit_mon; [..|done].
 Qed.
@@ -587,7 +615,11 @@ Typeclasses Opaque itree_impl_rel.
 Lemma itree_impl_rel_intro EV S σ P:
   σ -{mod_itree EV S }-> itree_impl_rel P →
   σ -{mod_itree EV S }-> P.
-Proof. move => ?. apply: steps_impl_mono; [done|]. move => ??? Hp. apply Hp. naive_solver. Qed.
+Proof. move => ?. apply: steps_impl_mono; [done|]. move => ??? Hp. apply Hp; [|done]. naive_solver. Qed.
+
+Ltac clear_itree :=
+  try match goal with | |- itree_rel _ _ _ => move => ?/=? end;
+  repeat match goal with | H : eqit _ _ _ ?t _ |- _ => clear H; clear t end.
 
 (** * Derived notions *)
 Definition TVis {EV S} (e : EV) : itree (moduleE EV S) unit :=
@@ -619,6 +651,12 @@ Definition TPut {EV S} (s : S) : itree (moduleE EV S) unit :=
   trigger (EPut s).
 
 (** * tsim *)
+Global Instance tsim_itree_l_proper EV S m1 n b:
+  Proper ((prod_relation (eqit eq false false) (=)) ==> (=) ==> (=) ==> iff) (tsim n b (mod_itree EV S) m1).
+Proof.
+  move => [??] [??] [/=Heq ->] ?? -> ?? ->.
+  split => Hsim ????; (eapply Hsim; [done|]). { by rewrite Heq. } { by rewrite -Heq. }
+Qed.
 
 Global Instance tsim_itree_r_proper EV S m1 b' n b:
   Proper ((=) ==> (=) ==> (prod_relation (eqit eq b' b') (=)) ==> iff) (tsim n b m1 (mod_itree EV S)).
@@ -627,326 +665,406 @@ Proof.
   split => Hsim ????. { rewrite -Heq. by eapply Hsim. } { rewrite Heq. by eapply Hsim. }
 Qed.
 
-(** * tstep *)
-Lemma eq_it_to_tstep_s {EV S} s t t' (Heqit : t ≈ t'):
-  TStepS (mod_itree EV S) (t, s) (λ G, G None (λ G', itree_rel G' (t', s))).
-Proof.
-  constructor => G HG. eexists _, _. split; [done|] => ? /= ?.
-  apply itree_rel_spec_intro. setoid_rewrite Heqit. by apply steps_spec_end.
-Qed.
-
-Lemma eq_it_to_tstep_i {EV S} s t t' (Heqit : t ≈ t'):
-  TStepI (mod_itree EV S) (t, s) (λ G, G false None (λ G', itree_rel G' (t', s))).
-Proof.
-  constructor => G HG. apply itree_impl_rel_intro. setoid_rewrite Heqit. apply steps_impl_end.
-  move => ?? Ht. eexists _, _. naive_solver.
-Qed.
-
-(** These step rules should always apply to itree with a bind at the
-top-level and discriminate on the argument of the bind.
-TODO: add a step rule that adds a bind a the top-level if there is none.  *)
-Program Definition itree_step_bind_s {EV S} A B s h (k : A → itree _ B) t :=
-  @eq_it_to_tstep_s EV S s (ITree.bind (ITree.bind t k) h)
-                    (ITree.bind t (fun r => ITree.bind (k r) h)) _.
-Next Obligation. move => *. by rewrite bind_bind. Qed.
-Global Hint Resolve itree_step_bind_s : tstep.
-
-Program Definition itree_step_bind_i {EV S} A B s h (k : A → itree _ B) t :=
-  @eq_it_to_tstep_i EV S s (ITree.bind (ITree.bind t k) h)
-                    (ITree.bind t (fun r => ITree.bind (k r) h)) _.
-Next Obligation. move => *. by rewrite bind_bind. Qed.
-Global Hint Resolve itree_step_bind_i : tstep.
-
-Program Definition itree_step_Ret_s EV S A (x : A) h s :=
-  @eq_it_to_tstep_s EV S s (ITree.bind (Ret x) h) (h x) _.
-Next Obligation. move => *. by rewrite bind_ret_l. Qed.
-Global Hint Resolve itree_step_Ret_s : tstep.
-
-Program Definition itree_step_Ret_i EV S A (x : A) h s :=
-  @eq_it_to_tstep_i EV S s (ITree.bind (Ret x) h) (h x) _.
-Next Obligation. move => *. by rewrite bind_ret_l. Qed.
-Global Hint Resolve itree_step_Ret_i : tstep.
-
-Program Definition itree_step_Tau_s EV S t s :=
-  @eq_it_to_tstep_s EV S s (Tau t) t _.
-Next Obligation. move => *. by rewrite tau_eutt. Qed.
-Global Hint Resolve itree_step_Tau_s : tstep.
-
-Lemma itree_step_Tau_i EV S k s:
-  TStepI (mod_itree EV S) (Tau k, s) (λ G, G true None (λ G', G' (k, s))).
-Proof.
-  constructor => ??. apply: steps_impl_step_end => ???.
-  invert_all @m_step; simplify_eq/=. eexists _, _. naive_solver.
-Qed.
-Global Hint Resolve itree_step_Tau_i : tstep.
-
-Lemma itree_step_Vis_s EV S k s e:
-  TStepS (mod_itree EV S) (TVis e;;;; k, s) (λ G, G (Some e) (λ G', itree_rel G' (k, s))).
-Proof.
-  constructor => ??. eexists _, _. split; [done|] => ? /= ?.
-  apply itree_rel_spec_intro. rewrite bind_trigger.
-  apply: steps_spec_step_end. { by econs. } naive_solver.
-Qed.
-Global Hint Resolve itree_step_Vis_s : tstep.
-
-Lemma itree_step_Vis_i EV S k s e:
-  TStepI (mod_itree EV S) (TVis e;;;; k, s) (λ G, G true (Some e) (λ G', itree_rel G' (k, s))).
-Proof.
-  constructor => ??. apply: steps_impl_step_end => ???.
-  invert_all @m_step; simplify_eq/=. cbn in H3; simplify_eq; simplify_K.
-  eexists _, _. split_and!; [done..|]. move => /= ? HG. eexists _. split; [done|].
-  apply HG => /=. by setoid_rewrite bind_ret_l.
-Qed.
-Global Hint Resolve itree_step_Vis_i : tstep.
-
-Lemma itree_step_Get_s EV S k s:
-  TStepS (mod_itree EV S) (x ← TGet;;; k x, s) (λ G, G None (λ G', itree_rel G' (k s, s))).
-Proof.
-  constructor => ??. eexists _, _. split; [done|] => ? /= ?.
-  apply itree_rel_spec_intro. rewrite bind_trigger.
-  apply: steps_spec_step_end. { by econs. } naive_solver.
-Qed.
-Global Hint Resolve itree_step_Get_s : tstep.
-
-Lemma itree_step_Get_i EV S k s:
-  TStepI (mod_itree EV S) (x ← TGet;;; k x, s) (λ G, G true None (λ G', itree_rel G' (k s, s))).
-Proof.
-  constructor => ??. apply: steps_impl_step_end => ???.
-  invert_all @m_step; simplify_eq/=. cbn in H3; simplify_eq; simplify_K.
-  eexists _, _. split_and!; [done..|]. move => /= ? HG. eexists _. split; [done|].
-  apply HG => /=. by setoid_rewrite bind_ret_l.
-Qed.
-Global Hint Resolve itree_step_Get_i : tstep.
-
-Lemma itree_step_Put_s EV S k s s':
-  TStepS (mod_itree EV S) (TPut s';;;; k, s) (λ G, G None (λ G', itree_rel G' (k, s'))).
-Proof.
-  constructor => ??. eexists _, _. split; [done|] => ? /= ?.
-  apply itree_rel_spec_intro. rewrite bind_trigger.
-  apply: steps_spec_step_end. { by econs. } naive_solver.
-Qed.
-Global Hint Resolve itree_step_Put_s : tstep.
-
-Lemma itree_step_Put_i EV S k s s':
-  TStepI (mod_itree EV S) (TPut s';;;; k, s) (λ G, G true None (λ G', itree_rel G' (k, s'))).
-Proof.
-  constructor => ??. apply: steps_impl_step_end => ???.
-  invert_all @m_step; simplify_eq/=. cbn in H3; simplify_eq; simplify_K.
-  eexists _, _. split_and!; [done..|]. move => /= ? HG. eexists _. split; [done|].
-  apply HG => /=. by setoid_rewrite bind_ret_l.
-Qed.
-Global Hint Resolve itree_step_Put_i : tstep.
-
-Lemma itree_step_All_s EV S T k s:
-  TStepS (mod_itree EV S) (x ← TAll T;;; k x, s) (λ G, G None (λ G', ∀ x, itree_rel G' (k x, s))).
-Proof.
-  constructor => ?. eexists _, _. split; [done|] => ? /= ?.
-  apply itree_rel_spec_intro. rewrite bind_trigger.
-  apply: steps_spec_step_end. { by econs. } naive_solver.
-Qed.
-Global Hint Resolve itree_step_All_s : tstep.
-
-Lemma itree_step_All_i EV S T k s:
-  TStepI (mod_itree EV S) (x ← TAll T;;; k x, s) (λ G, G true None (λ G', ∃ x, itree_rel G' (k x, s))).
-Proof.
-  constructor => ??. apply: steps_impl_step_end => ???.
-  invert_all @m_step; simplify_eq/=. cbn in H3; simplify_eq; simplify_K.
-  eexists _, _. split_and!; [done..|]. move => /= ? [? HG]. eexists _. split; [naive_solver|].
-  apply HG => /=. by setoid_rewrite bind_ret_l.
-Qed.
-Global Hint Resolve itree_step_All_i : tstep.
-
-Lemma itree_step_Exist_s EV S T k s:
-  TStepS (mod_itree EV S) (x ← TExist T;;; k x, s)
-            (λ G, G None (λ G', ∃ x, itree_rel G' (k x, s))).
-Proof.
-  constructor => ??. eexists _, _. split; [done|] => ? /= [??].
-  apply itree_rel_spec_intro. rewrite bind_trigger.
-  apply: steps_spec_step_end. { by econs. } naive_solver.
-Qed.
-Global Hint Resolve itree_step_Exist_s : tstep.
-
-Lemma itree_step_Exist_i EV S T k s:
-  TStepI (mod_itree EV S) (x ← TExist T;;; k x, s)
-            (λ G, G true None (λ G', ∀ x, itree_rel G' (k x, s))).
-Proof.
-  constructor => ??. apply: steps_impl_step_end => ???.
-  invert_all @m_step; simplify_eq/=. cbn in H3; simplify_eq; simplify_K.
-  eexists _, _. split_and!; [done..|]. move => /= ? HG. eexists _. split; [done|].
-  apply: HG => /=. by setoid_rewrite bind_ret_l.
-Qed.
-Global Hint Resolve itree_step_Exist_i : tstep.
-
-Lemma itree_step_Ub_s EV S T (k : T → _) s:
-  TStepS (mod_itree EV S) (x ← TUb;;; k x, s) (λ G, G None (λ G', True)).
-Proof.
-  constructor => ??. eexists _, _. split; [done|] => ? /= ?.
-  apply itree_rel_spec_intro. rewrite /TUb bind_bind bind_trigger.
-  apply: steps_spec_step_end. { by econs. } move => ? [[]?].
-Qed.
-Global Hint Resolve itree_step_Ub_s : tstep.
-
-Lemma itree_step_Nb_i EV S T (k : T → _) s:
-  TStepI (mod_itree EV S) (x ← TNb;;; k x, s) (λ G, G true None (λ G', True)).
-Proof.
-  constructor => ??. apply: steps_impl_step_end => ???.
-  invert_all @m_step; simplify_eq/=. cbn in H3; simplify_eq; simplify_K. destruct x.
-Qed.
-Global Hint Resolve itree_step_Nb_i : tstep.
-
-Lemma itree_step_Assume_s EV S P k s:
-  TStepS (mod_itree EV S) (TAssume P;;;; k, s) (λ G, G None (λ G', P → itree_rel G' (k, s))).
-Proof.
-  constructor => ??. eexists _, _. split; [done|] => ? /= ?.
-  apply itree_rel_spec_intro. rewrite /TAssume bind_bind bind_trigger.
-  apply: steps_spec_step_end. { by econs. } move => [??] [[??]?]; simplify_eq.
-  rewrite bind_ret_l. naive_solver.
-Qed.
-Global Hint Resolve itree_step_Assume_s : tstep.
-
-Lemma itree_step_Assume_i EV S P k s:
-  TStepI (mod_itree EV S) (TAssume P;;;; k, s) (λ G, G true None (λ G', P ∧ itree_rel G' (k, s))).
-Proof.
-  constructor => ??. apply: steps_impl_step_end => ???.
-  invert_all @m_step; simplify_eq/=. cbn in H3; simplify_eq; simplify_K.
-  eexists _, _. split_and!; [done..|]. move => /= ? [? HG]. eexists _. split; [naive_solver|].
-  apply: HG => /=. setoid_rewrite bind_ret_l. setoid_rewrite bind_ret_l. done.
-  Unshelve. done.
-Qed.
-Global Hint Resolve itree_step_Assume_i : tstep.
-
-Lemma itree_step_Assert_s EV S P k s:
-  TStepS (mod_itree EV S) (TAssert P;;;; k, s) (λ G, G None (λ G', P ∧ itree_rel G' (k, s))).
-Proof.
-  constructor => ??. eexists _, _. split; [done|] => ? /= [??].
-  apply itree_rel_spec_intro. rewrite /TAssert bind_bind bind_trigger.
-  apply: steps_spec_step_end. { by econs. } move => [??] [??]; simplify_eq.
-  rewrite bind_ret_l. naive_solver. Unshelve. by constructor.
-Qed.
-Global Hint Resolve itree_step_Assert_s : tstep.
-
-Lemma itree_step_Assert_i EV S P k s:
-  TStepI (mod_itree EV S) (TAssert P;;;; k, s) (λ G, P → G true None (λ G', itree_rel G' (k, s))).
-Proof.
-  constructor => ??. apply: steps_impl_step_end => ???.
-  invert_all @m_step; simplify_eq/=. cbn in H3; simplify_eq; simplify_K. destruct x.
-  eexists _, _. split_and!; [naive_solver..|]. move => /= ? HG. eexists _. split; [naive_solver|].
-  apply: HG => /=. setoid_rewrite bind_ret_l. setoid_rewrite bind_ret_l. done.
-Qed.
-Global Hint Resolve itree_step_Assert_i : tstep.
-
-Lemma itree_step_AssumeOpt_s EV S A (o : option A) k s:
-  TStepS (mod_itree EV S) (x ← TAssumeOpt o;;; k x, s) (λ G, G None (λ G', ∀ x, (o = Some x) → itree_rel G' (k x, s))).
-Proof.
-  constructor => ??. eexists _, _. split; [done|] => ? /= ?.
-  apply itree_rel_spec_intro. rewrite /TAssume bind_bind bind_trigger.
-  apply: steps_spec_step_end. { by econs. } move => [??] [[??]?]; simplify_eq.
-  rewrite bind_ret_l. naive_solver.
-Qed.
-Global Hint Resolve itree_step_AssumeOpt_s : tstep.
-
-Lemma itree_step_AssumeOpt_i EV S A (o : option A) k s:
-  TStepI (mod_itree EV S) (x ← TAssumeOpt o;;; k x, s) (λ G, G true None (λ G', ∃ x, o = Some x ∧ itree_rel G' (k x, s))).
-Proof.
-  constructor => ??. apply: steps_impl_step_end => ???.
-  invert_all @m_step; simplify_eq/=. cbn in H3; simplify_eq; simplify_K.
-  eexists _, _. split_and!; [naive_solver..|]. move => /= ? [? [? HG]]. subst.
-  eexists _. split; [naive_solver|]. apply: HG => /=. setoid_rewrite bind_ret_l. setoid_rewrite bind_ret_l.
-  Unshelve. 2: { by econstructor. } done.
-Qed.
-Global Hint Resolve itree_step_AssumeOpt_i : tstep.
-
-Lemma itree_step_AssertOpt_s EV S A (o : option A) k s:
-  TStepS (mod_itree EV S) (x ← TAssertOpt o;;; k x, s) (λ G, G None (λ G', ∃ x, o = Some x ∧ itree_rel G' (k x, s))).
-Proof.
-  constructor => ??. subst. eexists _, _. split; [done|] => ? /= [?[??]].
-  apply itree_rel_spec_intro. rewrite /TAssert bind_bind bind_trigger.
-  apply: steps_spec_step_end. { by econs. } Unshelve. 3: by econstructor. move => [??] [??]; simplify_eq.
-  rewrite bind_ret_l. naive_solver.
-Qed.
-Global Hint Resolve itree_step_AssertOpt_s : tstep.
-
-Lemma itree_step_AssertOpt_i EV S A (o : option A) k s:
-  TStepI (mod_itree EV S) (x ← TAssertOpt o;;; k x, s) (λ G, ∀ x, o = Some x → G true None (λ G', itree_rel G' (k x, s))).
-Proof.
-  constructor => ??. apply: steps_impl_step_end => ???.
-  invert_all @m_step; simplify_eq/=. cbn in H3; simplify_eq; simplify_K. destruct x.
-  eexists _, _. split_and!; [naive_solver..|]. move => /= ? HG. subst.
-  eexists _. split; [naive_solver|]. apply: HG => /=. setoid_rewrite bind_ret_l. by setoid_rewrite bind_ret_l.
-Qed.
-Global Hint Resolve itree_step_AssertOpt_i : tstep.
-
-Program Definition itree_step_recursive_bind_translate_s EV S R Q A B (f : A → itree (callE A B +' _) _) (t : itree (moduleE EV S) R) (k : R → itree (_ +' moduleE EV S) Q) h s :=
-  @eq_it_to_tstep_s EV S s (x ← interp (recursive f) (ITree.bind (translate inr_ t) k);;; h x)
-                    (ITree.bind t (fun r => x ← interp (recursive f) (k r);;; h x))_.
-Next Obligation. move => *. by rewrite interp_bind bind_bind interp_translate /= interp_trigger_h. Qed.
-Global Hint Resolve itree_step_recursive_bind_translate_s : tstep.
-
-Program Definition itree_step_recursive_translate_s EV S R A B (f : A → itree (callE A B +' _) _) (t : itree (moduleE EV S) R) h s :=
-  @eq_it_to_tstep_s EV S s (x ← interp (recursive f) (translate inr_ t);;; h x) (x ← t;;; h x) _.
-Next Obligation. move => *. by rewrite interp_translate /= interp_trigger_h. Qed.
-Global Hint Resolve itree_step_recursive_translate_s : tstep.
-
-Program Definition itree_step_recursive_call_s EV S R A B (f : A → itree (callE A B +' _) _) k (h : R → _) s a :=
-  @eq_it_to_tstep_s EV S s (x ← interp (recursive f) (y ← call a;;; k y);;; h x)
-            (y ← rec f a;;; x ← interp (recursive f) (k y);;; h x) _.
-Next Obligation. move => *. by rewrite interp_bind interp_recursive_call bind_bind. Qed.
-Global Hint Resolve itree_step_recursive_call_s : tstep.
-
-Program Definition itree_step_interp_ret_s EV S R E  (f : E ~> itree (moduleE EV S)) (a : R) h s :=
-  @eq_it_to_tstep_s EV S s (x ← interp f (Ret a);;; h x) (h a) _.
-Next Obligation. move => *. by rewrite interp_ret bind_ret_l. Qed.
-Global Hint Resolve itree_step_interp_ret_s : tstep.
-
-
 Lemma tsim_remember_rec {EV S A B} {mi : module EV} (PRE : _ → _ → _ → Prop)
       (POST : _ → _ → _ → Prop) (a : A) σi r (h : B → _) s n b:
   PRE a σi s →
   (∀ σi' y s', POST σi' y s' → σi' ⪯{mi, mod_itree EV S, n, b} (h y, s')) →
-  (∀ n, Plater (λ b', ∀ σi s h' a, PRE a σi s →
-         (∀ σi' y s', POST σi' y s' → σi' ⪯{mi, mod_itree EV S, n, b} (h' y, s')) →
-         σi ⪯{mi, mod_itree EV S, n, b'} ((y ← rec r a;;; h' y), s))) →
+  (∀ n', tiS?b n' ⊆ n →
+     Plater (λ b', ∀ σi s h' a, PRE a σi s →
+         (∀ σi' y s', POST σi' y s' → σi' ⪯{mi, mod_itree EV S, n', b} (h' y, s')) →
+         σi ⪯{mi, mod_itree EV S, n', b'} ((y ← rec r a;;; h' y), s))) →
   σi ⪯{mi, mod_itree EV S, n, b} (y ← rec r a;;; h y, s).
 Proof.
   move => ? Hh Hsim x.
   eapply (tsim_remember (ms:=mod_itree _ _)
     (λ n σi '(σt, s), ∃ a h', PRE a σi s ∧ σt = (y ← rec r a;;; h' y) ∧
       ∀ σi' y s', POST σi' y s' → σi' ⪯{mi, mod_itree EV S, n, b} (h' y, s'))). { naive_solver. }
-  { move => ???[??]? [?[?[?[?{}Hh]]]]. simplify_eq. eexists _, _. split_and!; [done..|] => ????.
-    apply: tsim_mono; [naive_solver|]. by apply ti_lt_impl_le. }
-  move => n' IH ?[??] [?[?[?[??]]]]. simplify_eq.
-  apply: Hsim; [|done..].
+  { move => ???[??]? [?[?[?[?{}Hh]]]]. simplify_eq. split!; [done..|] => ????.
+    apply: tsim_mono; [naive_solver|]. etrans; [|done]. apply ti_le_S_maybe. }
+  move => n' ? IH ?[??] [?[?[?[??]]]]. simplify_eq.
+  apply: Hsim; [done| |done..].
   naive_solver.
 Qed.
 
-Require refframe.example_modules.
-Module itree_examples.
-Import refframe.example_modules.
+(** * tstep *)
+(** ** typeclasses and infrastructure *)
+Class ITreeEq {E R} (b : bool) (t t' : itree E R) := {
+  itree_eq_proof : eqit eq true b t t'
+}.
+Global Hint Mode ITreeEq + + + ! - : tstep.
+Lemma ITreeEq_refl {E R} b (t : itree E R) :
+  ITreeEq b t t.
+Proof. done. Qed.
+Lemma ITreeEq_true {E R} b1 b2 (t t' : itree E R) :
+  eqit eq b1 b2 t t' →
+  ITreeEq true t t'.
+Proof. move => ?. constructor. by apply: eqit_mon; [..|done]. Qed.
+Lemma ITreeEq_false {E R} b1 (t t' : itree E R) :
+  eqit eq b1 false t t' →
+  ITreeEq false t t'.
+Proof. move => ?. constructor. by apply: eqit_mon; [..|done]. Qed.
 
-Lemma itree_trefines_tau_l :
-  trefines (MS (mod_itree nat unit) (Tau (Ret tt), tt)) (MS (mod_itree nat unit) (Ret tt, tt)).
-Proof. constructor => /= ?. rewrite tau_eutt. done. Qed.
+Global Hint Extern 5 (ITreeEq _ ?t _) => (assert_fails (is_var t); by apply ITreeEq_refl) : tstep.
+Global Hint Extern 10 (ITreeEq true _ _) => (refine (ITreeEq_true _ _ _ _ _); eassumption) : tstep.
+Global Hint Extern 10 (ITreeEq false _ _) => (refine (ITreeEq_false _ _ _ _); eassumption) : tstep.
 
-Lemma mod1_trefines_itree :
-  trefines (MS mod1 0) (MS (mod_itree nat unit) ((_ ← trigger (EVis 1) ;;; Ret tt), tt)).
+Class ITreeTStep {EV S} (cont b : bool) (t t' : itree (moduleE EV S) unit) := {
+  itree_tstep_proof : eqit eq true b t t'
+}.
+Global Hint Mode ITreeTStep + + + + ! - : tstep.
+
+Class ITreeTStepS {EV S} (t : itree (moduleE EV S) unit) (s : S) (κ : option EV)
+  (P : (itree (moduleE EV S) () → S → Prop) → Prop) := {
+    itree_tsteps_proof G:
+    P (λ t' s', itree_rel true G (t', s')) →
+    (t, s) -{ mod_itree EV S, κ }->ₛ itree_rel true G
+}.
+Global Hint Mode ITreeTStepS + + ! ! - - : tstep.
+
+Lemma itree_step_s_itree_step_cont EV S t t' (s : S) (κ : option EV) P `{!ITreeTStep true true t t'}
+      `{!ITreeTStepS t' s κ P} :
+  ITreeTStepS t s κ P.
+Proof. constructor => ??. move: ITreeTStep0 => [->]. by apply itree_tsteps_proof. Qed.
+Global Hint Resolve itree_step_s_itree_step_cont | 50 : tstep.
+
+Lemma itree_step_s_itree_step_no_cont EV S t t' (s : S) `{!ITreeTStep false true t t'}:
+  ITreeTStepS t s (@None EV) (λ G, G t' s).
+Proof. constructor => ??. move: ITreeTStep0 => [->]. by apply steps_spec_end. Qed.
+Global Hint Resolve itree_step_s_itree_step_no_cont | 100 : tstep.
+
+Lemma itree_tstep_s {EV S} s t t' κ `{!ITreeEq true t t'} `{!ITreeTStepS t' s κ P}:
+  TStepS (mod_itree EV S) (t, s) (λ G, G κ (λ G', P (λ t'' s', itree_rel true G' (t'', s')))).
 Proof.
-  constructor => /= ? Ht.
-  thas_trace_inv Ht. { tend. }
-  invert_all @m_step. revert select (_ ⊆ _) => <-.
-  rewrite bind_trigger. apply thas_trace_Vis.
-  thas_trace_inv. { tend. }
-  invert_all @m_step.
+  constructor => G HG. eexists _, _. split; [done|] => ? /= ?.
+  apply itree_rel_spec_intro. move: ITreeEq0 => [->]. by apply: itree_tsteps_proof.
 Qed.
+Global Hint Resolve itree_tstep_s : tstep.
 
-Lemma itree_trefines_mod1 :
-  trefines (MS (mod_itree nat unit) ((trigger (EVis 1);;;; Ret tt), tt)) (MS mod1 0).
+Class ITreeTStepI {EV S} (t : itree (moduleE EV S) unit) (s : S)
+      (P : (bool → option EV → ((itree (moduleE EV S) () → S → Prop) → Prop) → Prop) → Prop) := {
+    itree_tstepi_proof G:
+    P G →
+    (t, s) -{ mod_itree EV S }-> (λ b κ Pσ, ∃ (b' : bool) P', G b' κ P' ∧ (b' → b) ∧ ∀ G', P' G' → ∃ t t' s, Pσ (t, s) ∧ eqit eq true false t t' ∧ G' t' s)
+}.
+Global Hint Mode ITreeTStepI + + ! ! - : tstep.
+
+Lemma itree_step_i_itree_step_cont EV S t t' (s : S) P `{!ITreeTStep true false t t'}
+      `{!ITreeTStepI t' s P} :
+  ITreeTStepI (EV:=EV) t s P.
 Proof.
-  constructor => /= ?. rewrite bind_trigger => /(thas_trace_Vis_inv _ _ _ _)Ht.
-  apply: thas_trace_under_tall; [done..|] => {Ht} ? [?|?]; destruct_all?. { tend. }
-  revert select (_ ⊆ _) => <-.
-  tstep_Some; [by econs|] => ? ->.
-  move: H0 => /(thas_trace_Ret_inv _ _ _ _)Ht.
-  apply: thas_trace_under_tall; [done..|] => {Ht} ?/=?; destruct_all?. tend.
+  constructor => ??. apply itree_impl_rel_intro.
+  move: ITreeTStep0 => [->].
+  apply: steps_impl_mono; [by apply itree_tstepi_proof|].
+  move => /= * ?? HP ?. destruct_all?; simplify_eq. eexists _, _. split_and!; [done|naive_solver|].
+  move => ? /H2[?[?[? [/HP[?[??]] [? HG]]]]]. eexists _, _, _. split_and!; [done| |done].
+  etrans; [|done]. apply eqit_flip. by apply: eqit_mon; [..|done].
 Qed.
+Global Hint Resolve itree_step_i_itree_step_cont | 50 : tstep.
 
-End itree_examples.
+Lemma itree_step_i_itree_step_no_cont EV S t t' (s : S) `{!ITreeTStep false false t t'} :
+  ITreeTStepI (EV:=EV) t s (λ G, G false None (λ G', G' t' s)).
+Proof.
+  constructor => ??. apply steps_impl_end. eexists _, _. split_and!; [done..|].
+  move => /=??. eexists _, _, _. split_and!; [done| |done].
+  apply itree_tstep_proof.
+Qed.
+Global Hint Resolve itree_step_i_itree_step_no_cont | 100 : tstep.
+
+Lemma itree_tstep_i {EV S} s t t' `{!ITreeEq false t t'} `{!ITreeTStepI t' s P}:
+  TStepI (mod_itree EV S) (t, s) (λ G, P (λ b κ P', G b κ (λ G', P' (λ t'' s', itree_rel false G' (t'', s'))))).
+Proof.
+  constructor => ??. apply itree_impl_rel_intro.
+  move: ITreeEq0 => [->].
+  apply: steps_impl_mono; [by apply itree_tstepi_proof|].
+  move => /= * ?? HP ?. destruct_all?; simplify_eq. eexists _, _. split_and!; [done|naive_solver|].
+  move => ? /H2[?[?[? [/HP[?[??]] [? HG]]]]]. eexists (_, _). split; [done|]. apply HG. etrans; [|done].
+  apply eqit_flip. by apply: eqit_mon; [..|done].
+Qed.
+Global Hint Resolve itree_tstep_i : tstep.
+
+(** ** instances *)
+Lemma itree_tstep_bind {EV S} A B h (k : A → itree _ B) (t : itree (moduleE EV S) _) cont b:
+  ITreeTStep cont b (ITree.bind (ITree.bind t k) h) (ITree.bind t (fun r => ITree.bind (k r) h)).
+Proof. constructor. by rewrite bind_bind. Qed.
+Global Hint Resolve itree_tstep_bind : tstep.
+
+Lemma itree_tstep_ret {EV S} A h (x : A) cont b:
+  ITreeTStep (EV:=EV) (S:=S) cont b (ITree.bind (Ret x) h) (h x).
+Proof. constructor. by rewrite bind_ret_l. Qed.
+Global Hint Resolve itree_tstep_ret : tstep.
+
+Lemma itree_tstep_forever EV S R (t : itree (moduleE EV S) R) b:
+  ITreeTStep false b (ITree.forever t) (t;;;; ITree.forever t).
+Proof.
+  constructor. setoid_rewrite unfold_forever at 1.
+  apply: eqit_bind'; [done|]. move => ???.
+  by apply eqit_Tau_l.
+Qed.
+Global Hint Resolve itree_tstep_forever : tstep.
+
+Lemma itree_step_recursive_bind_bind_s EV S R A B C D (f : A → itree (callE A B +' _) _) t (j : C → _) (k : D → _) (h : R → _) cont b:
+  ITreeTStep (EV:=EV) (S:=S) cont b (x ← interp (recursive f) (y ← (z ← t;;; j z);;; k y);;; h x)
+                    (x ← interp (recursive f) (z ← t ;;;y ← j z;;; k y);;; h x).
+Proof. constructor. by rewrite bind_bind. Qed.
+Global Hint Resolve itree_step_recursive_bind_bind_s : tstep.
+
+Lemma itree_step_recursive_bind_ret_s EV S R A B D (f : A → itree (callE A B +' _) _) t (k : D → _) (h : R → _) cont b:
+  ITreeTStep (EV:=EV) (S:=S) cont b (x ← interp (recursive f) (y ← Ret t;;; k y);;; h x)
+                    (x ← interp (recursive f) (k t);;; h x).
+Proof. constructor. by rewrite bind_ret_l. Qed.
+Global Hint Resolve itree_step_recursive_bind_ret_s : tstep.
+
+Lemma itree_step_recursive_bind_translate_s EV S R Q A B (f : A → itree (callE A B +' _) _) (t : itree (moduleE EV S) R) (k : R → itree (_ +' moduleE EV S) Q) cont h:
+  ITreeTStep (EV:=EV) (S:=S) cont true (x ← interp (recursive f) (ITree.bind (translate inr_ t) k);;; h x)
+                    (ITree.bind t (fun r => x ← interp (recursive f) (k r);;; h x)).
+Proof. constructor. rewrite interp_bind bind_bind interp_translate /=/= interp_trigger_h. done. Qed.
+Global Hint Resolve itree_step_recursive_bind_translate_s : tstep.
+
+Lemma itree_step_recursive_translate_s EV S R A B (f : A → itree (callE A B +' _) _) (t : itree (moduleE EV S) R) h cont:
+  ITreeTStep (EV:=EV) (S:=S) cont true (x ← interp (recursive f) (translate inr_ t);;; h x)
+                    (x ← t;;; h x).
+Proof. constructor. by rewrite interp_translate /= interp_trigger_h. Qed.
+Global Hint Resolve itree_step_recursive_translate_s : tstep.
+
+Lemma itree_step_recursive_call_s EV S R A B (f : A → itree (callE A B +' _) _) k (h : R → _) a:
+  ITreeTStep (EV:=EV) (S:=S) false true (x ← interp (recursive f) (y ← call a;;; k y);;; h x)
+                    (y ← rec f a;;; x ← interp (recursive f) (k y);;; h x).
+Proof. constructor. by rewrite interp_bind interp_recursive_call bind_bind. Qed.
+Global Hint Resolve itree_step_recursive_call_s : tstep.
+
+Lemma itree_step_interp_ret_s EV S R E  (f : E ~> itree (moduleE EV S)) (a : R) h cont:
+  ITreeTStep (EV:=EV) (S:=S) cont true (x ← interp f (Ret a);;; h x) (h a).
+Proof. constructor. by rewrite interp_ret bind_ret_l. Qed.
+Global Hint Resolve itree_step_interp_ret_s : tstep.
+
+Lemma itree_tstep_Tau_s {EV S} t cont:
+  ITreeTStep (EV:=EV) (S:=S) cont true (Tau t) t.
+Proof. constructor. by rewrite tau_eutt. Qed.
+Global Hint Resolve itree_tstep_Tau_s : tstep.
+
+Lemma itree_step_Tau_i EV S t s:
+  ITreeTStepI (EV:=EV) (S:=S) (Tau t) s (λ G, G true None (λ G', G' t s)).
+Proof.
+  constructor => ??. apply: steps_impl_step_end => ???.
+  invert_all @m_step; simplify_eq/=. naive_solver.
+Qed.
+Global Hint Resolve itree_step_Tau_i : tstep.
+
+Lemma itree_step_Vis_s EV S k (s : S) (e : EV):
+  ITreeTStepS (r ← TVis e;;; k r) s (Some e) (λ G, G (k tt) s).
+Proof.
+  constructor => ??. rewrite bind_trigger.
+  apply: steps_spec_step_end. { by econs. } naive_solver.
+Qed.
+Global Hint Resolve itree_step_Vis_s : tstep.
+
+Lemma itree_step_Vis_i EV S k s e:
+  ITreeTStepI (EV:=EV) (S:=S) (r ← TVis e;;; k r) s (λ G, G true (Some e) (λ G', G' (k tt) s)).
+Proof.
+  constructor => ??. apply: steps_impl_step_end => ???.
+  invert_all @m_step; simplify_eq/=. cbn in H3; simplify_eq; simplify_K.
+  eexists _, _. split_and!; [done..|]. move => /= ? HG. eexists _, _, _. split_and!; [done| |done].
+  by setoid_rewrite bind_ret_l.
+Qed.
+Global Hint Resolve itree_step_Vis_i : tstep.
+
+Lemma itree_step_Get_s EV S k s:
+  ITreeTStepS (EV:=EV) (S:=S) (x ← TGet;;; k x) s None (λ G, G (k s) s).
+Proof.
+  constructor => ??. rewrite bind_trigger.
+  apply: steps_spec_step_end. { by econs. } naive_solver.
+Qed.
+Global Hint Resolve itree_step_Get_s : tstep.
+
+Lemma itree_step_Get_i EV S k s:
+  ITreeTStepI (EV:=EV) (S:=S) (x ← TGet;;; k x) s (λ G, G true None (λ G', G' (k s) s)).
+Proof.
+  constructor => ??. apply: steps_impl_step_end => ???.
+  invert_all @m_step; simplify_eq/=. cbn in H3; simplify_eq; simplify_K.
+  eexists _, _. split_and!; [done..|]. move => /= ? HG. eexists _, _, _. split_and!; [done| |done].
+  by setoid_rewrite bind_ret_l.
+Qed.
+Global Hint Resolve itree_step_Get_i : tstep.
+
+Lemma itree_step_Put_s EV S k s s':
+  ITreeTStepS (EV:=EV) (S:=S) (x ← TPut s';;; k x) s None (λ G, G (k tt) s').
+Proof.
+  constructor => ??. rewrite bind_trigger.
+  apply: steps_spec_step_end. { by econs. } naive_solver.
+Qed.
+Global Hint Resolve itree_step_Put_s : tstep.
+
+Lemma itree_step_Put_i EV S k s s':
+  ITreeTStepI (EV:=EV) (S:=S) (x ← TPut s';;; k x) s (λ G, G true None (λ G', G' (k tt) s')).
+Proof.
+  constructor => ??. apply: steps_impl_step_end => ???.
+  invert_all @m_step; simplify_eq/=. cbn in H3; simplify_eq; simplify_K.
+  eexists _, _. split_and!; [done..|]. move => /= ? HG. eexists _, _, _. split_and!; [done| |done].
+  by setoid_rewrite bind_ret_l.
+Qed.
+Global Hint Resolve itree_step_Put_i : tstep.
+
+Lemma itree_step_All_s EV S T k s:
+  ITreeTStepS (EV:=EV) (S:=S) (x ← TAll T;;; k x) s None (λ G, ∀ x, G (k x) s).
+Proof.
+  constructor => ??. rewrite bind_trigger.
+  apply: steps_spec_step_end. { by econs. } naive_solver.
+Qed.
+Global Hint Resolve itree_step_All_s : tstep.
+
+Lemma itree_step_All_i EV S T k s:
+  ITreeTStepI (EV:=EV) (S:=S) (x ← TAll T;;; k x) s (λ G, G true None (λ G', ∃ x, G' (k x) s)).
+Proof.
+  constructor => ??. apply: steps_impl_step_end => ???.
+  invert_all @m_step; simplify_eq/=. cbn in H3; simplify_eq; simplify_K.
+  eexists _, _. split_and!; [done..|]. move => /= ? [? HG]. eexists _, _, _. split_and!; [naive_solver| |done].
+  by setoid_rewrite bind_ret_l.
+Qed.
+Global Hint Resolve itree_step_All_i : tstep.
+
+Lemma itree_step_Exist_s EV S T k s:
+  ITreeTStepS (EV:=EV) (S:=S) (x ← TExist T;;; k x) s None (λ G, ∃ x, G (k x) s).
+Proof.
+  constructor => ? [??]. rewrite bind_trigger.
+  apply: steps_spec_step_end. { by econs. } naive_solver.
+Qed.
+Global Hint Resolve itree_step_Exist_s : tstep.
+
+Lemma itree_step_Exist_i EV S T k s:
+  ITreeTStepI (EV:=EV) (S:=S) (x ← TExist T;;; k x) s (λ G, ∀ x, G true None (λ G', G' (k x) s)).
+Proof.
+  constructor => ??. apply: steps_impl_step_end => ???.
+  invert_all @m_step; simplify_eq/=. cbn in H3; simplify_eq; simplify_K.
+  eexists _, _. split_and!; [done..|]. move => /= ? HG. eexists _, _, _. split_and!; [naive_solver| |done].
+  by setoid_rewrite bind_ret_l.
+Qed.
+Global Hint Resolve itree_step_Exist_i : tstep.
+
+Lemma itree_step_Ub_s EV S T (k : T → _) s:
+  ITreeTStepS (EV:=EV) (S:=S) (x ← TUb;;; k x) s None (λ G, True).
+Proof.
+  constructor => ??. rewrite /TUb bind_bind bind_trigger.
+  apply: steps_spec_step_end. { by econs. } move => /=? [[]?].
+Qed.
+Global Hint Resolve itree_step_Ub_s : tstep.
+
+Lemma itree_step_Ub_end_s EV S s:
+  ITreeTStepS (EV:=EV) (S:=S) TUb s None (λ G, True).
+Proof.
+  constructor => ??. rewrite /TUb bind_trigger.
+  apply: steps_spec_step_end. { by econs. } move => /=? [[]?].
+Qed.
+Global Hint Resolve itree_step_Ub_end_s : tstep.
+
+Lemma itree_step_Nb_i EV S T (k : T → _) s:
+  ITreeTStepI (EV:=EV) (S:=S) (x ← TNb;;; k x) s (λ G, G true None (λ G', True)).
+Proof.
+  constructor => ??. apply: steps_impl_step_end => ???.
+  invert_all @m_step; simplify_eq/=. cbn in H3; simplify_eq; simplify_K. destruct x.
+Qed.
+Global Hint Resolve itree_step_Nb_i : tstep.
+
+Lemma itree_step_Nb_end_i EV S s:
+  ITreeTStepI (EV:=EV) (S:=S) TNb s (λ G, G true None (λ G', True)).
+Proof.
+  constructor => ??. apply: steps_impl_step_end => ???.
+  invert_all @m_step; simplify_eq/=. cbn in H3; simplify_eq; simplify_K. destruct x.
+Qed.
+Global Hint Resolve itree_step_Nb_end_i : tstep.
+
+Lemma itree_step_Assume_s EV S P k s:
+  ITreeTStepS (EV:=EV) (S:=S) (x ← TAssume P;;; k x) s None (λ G, P → G (k tt) s).
+Proof.
+  constructor => ??. rewrite bind_bind bind_trigger. setoid_rewrite bind_ret_l.
+  apply: steps_spec_step_end. { by econs. } move => ? [[]]. naive_solver.
+Qed.
+Global Hint Resolve itree_step_Assume_s : tstep.
+
+Lemma itree_step_Assume_i EV S P k s:
+  ITreeTStepI (EV:=EV) (S:=S) (x ← TAssume P;;; k x) s (λ G, G true None (λ G', P ∧ G' (k tt) s)).
+Proof.
+  constructor => ??. apply: steps_impl_step_end => ???.
+  invert_all @m_step; simplify_eq/=. cbn in H3; simplify_eq; simplify_K.
+  eexists _, _. split_and!; [done..|]. move => /= ? [? HG]. eexists _, _, _. split_and!; [naive_solver| |done].
+  setoid_rewrite bind_ret_l. by setoid_rewrite bind_ret_l.
+  Unshelve. done.
+Qed.
+Global Hint Resolve itree_step_Assume_i : tstep.
+
+Lemma itree_step_Assert_s EV S P k s:
+  ITreeTStepS (EV:=EV) (S:=S) (x ← TAssert P;;; k x) s None (λ G, P ∧ G (k tt) s).
+Proof.
+  constructor => ?[??]. rewrite bind_bind bind_trigger. setoid_rewrite bind_ret_l.
+  apply: steps_spec_step_end. { by econs. } naive_solver.
+  Unshelve. done.
+Qed.
+Global Hint Resolve itree_step_Assert_s : tstep.
+
+Lemma itree_step_Assert_i EV S P k s:
+  ITreeTStepI (EV:=EV) (S:=S) (x ← TAssert P;;; k x) s (λ G, P → G true None (λ G', G' (k tt) s)).
+Proof.
+  constructor => ??. apply: steps_impl_step_end => ???.
+  invert_all @m_step; simplify_eq/=. cbn in H3; simplify_eq; simplify_K. destruct x.
+  eexists _, _. split_and!; [naive_solver|done..|].
+  move => /= ??. eexists _, _, _. split_and!; [naive_solver| |done].
+  setoid_rewrite bind_ret_l. by setoid_rewrite bind_ret_l.
+Qed.
+Global Hint Resolve itree_step_Assert_i : tstep.
+
+Lemma itree_step_AssumeOpt_s EV S T (o : option T) k s:
+  ITreeTStepS (EV:=EV) (S:=S) (x ← TAssumeOpt o;;; k x) s None (λ G, ∀ x, o = Some x → G (k x) s).
+Proof.
+  constructor => ??. rewrite bind_bind bind_trigger. setoid_rewrite bind_ret_l.
+  apply: steps_spec_step_end. { by econs. } move => ? [[]]. naive_solver.
+Qed.
+Global Hint Resolve itree_step_AssumeOpt_s : tstep.
+
+Lemma itree_step_AssumeOpt_i EV S T (o : option T) k s:
+  ITreeTStepI (EV:=EV) (S:=S) (x ← TAssumeOpt o;;; k x) s (λ G, G true None (λ G', ∃ x, o = Some x ∧ G' (k x) s)).
+Proof.
+  constructor => ??. apply: steps_impl_step_end => ???.
+  invert_all @m_step; simplify_eq/=. cbn in H3; simplify_eq; simplify_K.
+  eexists _, _. split_and!; [done..|]. move => /= ? [? [? HG]]. subst.
+  eexists _, _, _. split_and!; [naive_solver| |done].
+  setoid_rewrite bind_ret_l.
+  Unshelve. 2: { by econstructor. } by setoid_rewrite bind_ret_l.
+Qed.
+Global Hint Resolve itree_step_AssumeOpt_i : tstep.
+
+Lemma itree_step_AssertOpt_s EV S T (o : option T) k s:
+  ITreeTStepS (EV:=EV) (S:=S) (x ← TAssertOpt o;;; k x) s None (λ G, ∃ x, o = Some x ∧ G (k x) s).
+Proof.
+  constructor => ?[?[??]]. rewrite bind_bind bind_trigger. setoid_rewrite bind_ret_l.
+  apply: steps_spec_step_end. { by econs. } Unshelve. 3: by econstructor. move => [??] [??]; simplify_eq. done.
+Qed.
+Global Hint Resolve itree_step_AssertOpt_s : tstep.
+
+Lemma itree_step_AssertOpt_i EV S T (o : option T) k s:
+  ITreeTStepI (EV:=EV) (S:=S) (x ← TAssertOpt o;;; k x) s (λ G, ∀ x, o = Some x → G true None (λ G', G' (k x) s)).
+Proof.
+  constructor => ??. apply: steps_impl_step_end => ???.
+  invert_all @m_step; simplify_eq/=. cbn in H3; simplify_eq; simplify_K. destruct x.
+  eexists _, _. split_and!; [naive_solver|done..|].
+  move => /= ??. eexists _, _, _. split_and!; [naive_solver| |done].
+  setoid_rewrite bind_ret_l. by setoid_rewrite bind_ret_l.
+Qed.
+Global Hint Resolve itree_step_AssertOpt_i : tstep.
+
+Module itree_test.
+Local Definition test_itree : itree (moduleE _ _) ()
+  := ((s ← TGet;;; TPut (S s);;;; Ret tt) ;;;; TVis (1);;;; Ret tt);;;; TNb.
+Goal trefines (MS (mod_itree _ _) (test_itree, 0)) (MS (mod_itree _ _) (test_itree, 0)).
+  apply tsim_implies_trefines => ? /=. rewrite /test_itree.
+
+  tstep_i; clear_itree.
+  tstep_i; clear_itree.
+  tstep_i; clear_itree.
+  tstep_s; clear_itree.
+  tstep_s; clear_itree.
+  tstep_s; clear_itree.
+  split!. clear_itree.
+  tstep_s; clear_itree.
+  tstep_i; clear_itree.
+  done.
+Abort.
+End itree_test.
