theories/imp_to_asm_examples.v
@@ -1,0 +1,79 @@
+Require Export refframe.module.
+Require Import refframe.trefines.
+Require Import refframe.filter.
+Require Import refframe.product.
+Require Import refframe.seq_product.
+Require Import refframe.proof_techniques.
+Require Import refframe.imp.
+Require Import refframe.asm.
+Require Import refframe.itree.
+Require Import refframe.imp_to_asm.
+
+Local Open Scope Z_scope.
+
+Definition asm_add : gmap Z asm_instr :=
+  <[ 100 := [
+        (* add R0, R0, R1 *)
+        WriteReg "R0" (λ rs, rs !!! "R0" + rs !!! "R1");
+        WriteReg "PC" (λ rs, rs !!! "PC" + 4)
+    ] ]> $
+  <[ 104 := [
+        (* ret *)
+        WriteReg "PC" (λ rs, rs !!! "R30")
+    ] ]> $ ∅.
+
+Definition imp_add : fndef := {|
+  fd_args := ["a"; "b"];
+  fd_body := (BinOp (Var "a") AddOp (Var "b"));
+  fd_static := I
+|}.
+
+Definition imp_add_prog : gmap string fndef :=
+  <[ "add" := imp_add ]> ∅.
+
+Local Hint Constants Transparent : tstep.
+Local Ltac go := clear_itree; destruct_all?; simplify_eq/=.
+Local Ltac go_i := tstep_i; go.
+Local Ltac go_s := tstep_s; go.
+
+Lemma asm_add_refines_imp_add :
+  trefines (MS asm_module (initial_asm_state asm_add))
+           (MS (imp_to_asm imp_module) (initial_imp_to_asm_state imp_module (initial_imp_state imp_add_prog) {[ 100; 104 ]} {[ "add" ]} (<["add" := 100]> ∅))).
+Proof.
+  apply tsim_implies_trefines => /= n.
+
+  rewrite /initial_asm_state/initial_imp_state/initial_imp_to_asm_state.
+
+  tstep_i => ???? Hin. unfold asm_add in Hin.
+  go_s. go_s. eexists _; go. go_s. eexists _; go. go_s. split; [done|]. go.
+  go_s => b; go. destruct b. 2: { repeat (go_s; intros; go). }
+  go_s => r; go. go_s => f; go. go_s => vs; go.
+  go_s => ?; go. go_s => ?; go. go_s => ?; go. go_s => Hargs; go.
+  go_s. go_s. go_s.
+  have ?: f = "add" by set_solver. subst. simplify_map_eq.
+  change ((Waiting false)) with (expr_fill [] (Waiting false)).
+  tstep_s. split!; [|done|]; simplify_map_eq; [done|]. case_bool_decide.
+  2: { change (UbE) with (expr_fill [] UbE). tstep_s. done. }
+  destruct vs as [|v1 [|v2 []]] => //=.
+  move: Hargs => -[?[? /= Hregs]]. unfold saved_registers in *. decompose_Forall_hyps.
+  tstep_i. split; [done|].
+  tstep_i. split. { by simplify_map_eq. }
+  tstep_i => ??. simplify_map_eq. erewrite lookup_total_correct; [|by simplify_map_eq].
+  rewrite {1}/asm_add. simplify_map_eq.
+  tstep_i. split. { by simplify_map_eq. } simplify_map_eq.
+  tstep_i => ??. simplify_map_eq. erewrite lookup_total_correct; [|by simplify_map_eq].
+  case_match. 1: { admit. }
+  change (ReturnExt false (BinOp v1 AddOp v2)) with (expr_fill [ReturnExtCtx false] (BinOp v1 AddOp v2)).
+  go_s => n1 n2 ??; subst.
+  change (ReturnExt false (n1 + n2)) with (expr_fill [] (ReturnExt false (n1 + n2))).
+  go_s. go_s. eexists _; go. go_s. eexists _; go. go_s. eexists false; go.
+  go_s. eexists _; go. go_s. eexists _; go. go_s. eexists _; go.
+  go_s. go_s. split; [done|]; go. go_s. go_s. split; [shelve|]; go. go_s. split; [done|]. go.
+  go_s. split; [done|]. go.
+  Unshelve.
+  2: { unfold imp_to_asm_ret. unfold tmp_registers, saved_registers.
+       split!; decompose_Forall; simplify_map_eq => //.
+       all: try by apply lookup_lookup_total.
+       admit.
+  }
+Abort.
